upload rules cnf

Cnf.fst
@@ -1,6 +1,9 @@
 module Cnf
 
 open FStar.Math.Lib
+open FStar.Mul
+module L = FStar.List.Tot.Base
+open FStar.Ghost
 open FormulaT
 open Utils
 
@@ -57,4 +60,166 @@ let rec count_or_pairs (f:formula_t) (ors_above_left:nat) : Tot nat (decreases f
 
 
 let measure (f:formula_t) (h1:nat) (h2:nat)
-    = (weight_of_ands f, count_dimplies f, count_implies f, count_or_pairs f h1, count_and_pairs f h2)
+    : r : list nat {L.length r = 5}
+    = weight_of_ands f::(count_dimplies f::(count_implies f::(count_or_pairs f h1::[count_and_pairs f h2])))
+
+
+let apply_rule_1 (f:formula_t) (ors_above_left : erased nat) (ands_above_left : erased nat)
+    : Pure formula_t (requires valid_formula_t f && DImplies? f)
+                     (ensures fun r -> (valid_formula_t r /\ 
+                                        equivalent f r /\ 
+                                        weight_of_ands r <= weight_of_ands f /\ 
+                                        count_dimplies r < count_dimplies f /\
+                                        smaller (measure r ors_above_left ands_above_left) (measure f ors_above_left ands_above_left)))
+    = let DImplies f1 f2 = f in
+      let f11 = Implies f1 f2 in
+      let f12 = Implies f2 f1 in
+      let r = And f11 f12 in
+      assert (count_dimplies r = count_dimplies f11 + count_dimplies f12);
+      assert (count_dimplies r = 2 * (count_dimplies f1 + count_dimplies f2));
+      assert (count_dimplies f = 1 + pow2 (count_dimplies f1 + count_dimplies f2));
+      mult2_upper (count_dimplies f1 + count_dimplies f2);
+      r
+
+
+let apply_rule_2 (f:formula_t) (ors_above_left : erased nat) (ands_above_left : erased nat)
+    : Pure formula_t (requires valid_formula_t f && Implies? f)
+                     (ensures fun r -> (valid_formula_t r /\
+                                        equivalent f r /\
+                                        weight_of_ands r <= weight_of_ands f /\
+                                        count_dimplies r <= count_dimplies f /\
+                                        count_implies r < count_implies f /\
+                                        smaller (measure r ors_above_left ands_above_left) (measure f ors_above_left ands_above_left)))
+    = let Implies f1 f2 = f in
+      let r = Or (Not f1) f2 in
+    //   assert (weight_of_ands r <= weight_of_ands f);
+      r
+
+
+let apply_rule_3 (f:formula_t) (ors_above_left : erased nat) (ands_above_left : erased nat)
+    : Pure formula_t (requires valid_formula_t f && Or? f && And? (Or?.f2 f))
+                     (ensures fun r -> (valid_formula_t r /\
+                                        equivalent f r /\
+                                        weight_of_ands r < weight_of_ands f /\
+                                        smaller (measure r ors_above_left ands_above_left) (measure f ors_above_left ands_above_left)))
+    = let Or f1 f2 = f in
+      let And f21 f22 = f2 in
+      And (Or f1 f21) (Or f1 f22)
+
+
+let apply_rule_4 (f:formula_t) (ors_above_left : erased nat) (ands_above_left : erased nat)
+    : Pure formula_t (requires valid_formula_t f && Or? f && And? (Or?.f1 f))
+                     (ensures fun r -> (valid_formula_t r /\
+                                        equivalent f r /\
+                                        weight_of_ands r < weight_of_ands f /\
+                                        smaller (measure r ors_above_left ands_above_left) (measure f ors_above_left ands_above_left)))
+    = let Or f1 f2 = f in 
+      let And f11 f12 = f1 in
+      And (Or f11 f2) (Or f12 f2)
+
+
+let rule_5_prop_aux (f:formula_t) (ors_above_left:nat)
+    : Lemma (ensures count_or_pairs f ors_above_left <= count_or_pairs f (ors_above_left + 1))
+    = ()
+
+
+let rule_5_prop (f1:formula_t) (f2:formula_t) (f3:formula_t) (ors_above_left:nat)
+    : Lemma (ensures count_or_pairs (Or (Or f1 f2) f3) ors_above_left < count_or_pairs (Or f1 (Or f2 f3)) ors_above_left)
+    = assert (count_or_pairs (Or f1 (Or f2 f3)) ors_above_left = 
+              count_or_pairs f1 ors_above_left + 
+              count_or_pairs f2 (ors_above_left + 1) + 
+              count_or_pairs f3 (ors_above_left + 2) + 
+              ors_above_left + ors_above_left + 1);
+      assert (count_or_pairs (Or (Or f1 f2) f3) ors_above_left =
+              count_or_pairs f1 ors_above_left +
+              count_or_pairs f2 (ors_above_left + 1) +
+              count_or_pairs f3 (ors_above_left + 1) +
+              ors_above_left + ors_above_left);
+      rule_5_prop_aux f3 (ors_above_left + 1);
+      assert (count_or_pairs f3 (ors_above_left + 1) <= count_or_pairs f3 (ors_above_left + 2));
+      assert (count_or_pairs (Or (Or f1 f2) f3) ors_above_left < count_or_pairs (Or f1 (Or f2 f3)) ors_above_left)
+
+
+let apply_rule_5 (f:formula_t) (ors_above_left : erased nat) (ands_above_left : erased nat)
+    : Pure formula_t (requires valid_formula_t f && Or? f && Or? (Or?.f2 f))
+                     (ensures fun r -> (valid_formula_t r /\
+                                        equivalent f r /\
+                                        weight_of_ands r <= weight_of_ands f /\
+                                        count_dimplies r <= count_dimplies f /\
+                                        count_implies r <= count_implies f /\
+                                        count_or_pairs r ors_above_left < count_or_pairs f ors_above_left /\
+                                        smaller (measure r ors_above_left ands_above_left) (measure f ors_above_left ands_above_left)))
+    = let Or f1 f2 = f in 
+      let Or f21 f22 = f2 in
+      let r = Or (Or f1 f21) f22 in
+      rule_5_prop f1 f21 f22 ors_above_left;
+      assert (count_or_pairs r ors_above_left < count_or_pairs f ors_above_left);
+      r
+
+
+// let rule_6_prop_aux (f:formula_t) (ands_above_left:nat)
+//     : Lemma (ensures count_and_pairs f ands_above_left <= count_and_pairs f (ands_above_left + 1))
+//     = ()
+
+
+// let rule_6_prop (f1:formula_t) (f2:formula_t) (f3:formula_t) (ands_above_left:nat)
+//     : Lemma (ensures count_and_pairs (And (And f1 f2) f3) ands_above_left < count_and_pairs (And f1 (And f2 f3)) ands_above_left)
+//     = assert (count_and_pairs (And f1 (And f2 f3)) ands_above_left = 
+//               count_and_pairs f1 ands_above_left + 
+//               count_and_pairs f2 (ands_above_left + 1) +
+//               count_and_pairs f3 (ands_above_left + 2) +
+//               ands_above_left + ands_above_left + 1);
+//       assert (count_and_pairs (And (And f1 f2) f3) ands_above_left =
+//               count_and_pairs f1 ands_above_left +
+//               count_and_pairs f2 (ands_above_left + 1) +
+//               count_and_pairs f3 (ands_above_left + 1) +
+//               ands_above_left + ands_above_left);
+//       rule_6_prop_aux f3 (ands_above_left + 1);
+//       assert (count_and_pairs f3 (ands_above_left + 1) <= count_and_pairs f3 (ands_above_left + 2));
+//       assert (count_and_pairs (And (And f1 f2) f3) ands_above_left < count_and_pairs (And f1 (And f2 f3)) ands_above_left)
+
+
+// let apply_rule_6 (f:formula_t) (ors_above_left : erased nat) (ands_above_left : erased nat)
+//     : Pure formula_t (requires valid_formula_t f && And? f && And? (And?.f2 f))
+//                      (ensures fun r -> (valid_formula_t r /\
+//                                         equivalent f r /\
+//                                         weight_of_ands r <= weight_of_ands f /\
+//                                         count_dimplies r <= count_dimplies f /\
+//                                         count_implies r <= count_implies f /\
+//                                         count_or_pairs r ors_above_left <= count_or_pairs f ors_above_left /\
+//                                         count_and_pairs r ands_above_left < count_and_pairs f ands_above_left /\
+//                                         smaller (measure r ors_above_left ands_above_left) (measure f ors_above_left ands_above_left)))
+//     = let And f1 f2 = f in 
+//       let And f21 f22 = f2 in 
+//       let r = And (And f1 f21) f22 in
+//       rule_6_prop f1 f21 f22 ands_above_left;
+//       assert (count_and_pairs r ands_above_left < count_and_pairs f ands_above_left);
+//       r
+
+
+let rule_7_prop (f1:formula_t) (f2:formula_t)
+    : Lemma (requires weight_of_ands f1 >= 2 && weight_of_ands f2 >= 2)
+            (ensures weight_of_ands (And (Not f1) (Not f2)) < weight_of_ands (Not (Or f1 f2)))
+    = assert (weight_of_ands (And (Not f1) (Not f2)) = pow2 (weight_of_ands f1) + pow2 (weight_of_ands f2) + 1);
+      assert (weight_of_ands (Not (Or f1 f2)) = pow2 (weight_of_ands f1 * weight_of_ands f2));
+      if weight_of_ands f1 >= weight_of_ands f2 then
+        (
+          sumpow_upper (weight_of_ands f1) (weight_of_ands f2);
+          assert (pow2 (weight_of_ands f1) + pow2 (weight_of_ands f2) + 1 < pow2 (weight_of_ands f1 * weight_of_ands f2));
+          assert (weight_of_ands (And (Not f1) (Not f2)) < weight_of_ands (Not (Or f1 f2)))
+        )
+      else sumpow_upper (weight_of_ands f2) (weight_of_ands f1)
+
+
+let apply_rule_7 (f:formula_t) (ors_above_left : erased nat) (ands_above_left : erased nat)
+    : Pure formula_t (requires valid_formula_t f && Not? f && Or? (Not?.f f))
+                     (ensures fun r -> (valid_formula_t r /\
+                                        equivalent f r /\
+                                        weight_of_ands r < weight_of_ands f /\
+                                        smaller (measure r ors_above_left ands_above_left) (measure f ors_above_left ands_above_left)))
+    = let Not f1 = f in
+      let Or f11 f12 = f1 in
+      let r = And (Not f11) (Not f12) in
+      rule_7_prop f11 f12;
+      assert (weight_of_ands r < weight_of_ands f);
+      r
