Utils.fst
@@ -1,6 +1,7 @@
 module Utils
 
 module L = FStar.List.Tot.Base
+open FStar.Mul
 
 
 let rec my_nth (#a:Type) (l : list a) (n:int {n >= 0 && n < L.length l}) : a
@@ -12,8 +13,54 @@ let integer_to_char_sequence (x:int) : list FStar.String.char
     = FStar.String.list_of_string (string_of_int x)
 
 
-// let rec n_falses (n:int)
-//     : Pure (list bool) (requires n >= 0)
-//                        (ensures fun r -> L.length r = n)
-//     = if n = 0 then []
-//       else L.append (n_falses (n - 1)) [false]
+let rec n_falses (n:int)
+    : Pure (list bool) (requires n >= 0)
+                       (ensures fun r -> L.length r = n)
+    = if n = 0 then []
+      else false::(n_falses (n - 1))
+
+
+let smaller (a : list nat) (b : list nat {L.length a = L.length b && L.length a = 5})
+    : bool
+    = L.hd a < L.hd b ||
+      (L.hd a <= L.hd b && my_nth a 1 < my_nth b 1) ||
+      (L.hd a <= L.hd b && my_nth a 1 <= my_nth b 1 && my_nth a 2 < my_nth b 2) ||
+      (L.hd a <= L.hd b && my_nth a 1 <= my_nth b 1 && my_nth a 2 <= my_nth b 2 &&  my_nth a 3 < my_nth b 3) ||
+      (L.hd a <= L.hd b && my_nth a 1 <= my_nth b 1 && my_nth a 2 <= my_nth b 2 &&  my_nth a 3 <= my_nth b 3 && my_nth a 4 < my_nth b 4)
+
+
+let rec mult2_upper (x:int)
+    : Lemma (requires x >= 0)
+            (ensures 2 * x < 1 + pow2 x)
+    = if x = 0 then ()
+      else mult2_upper (x - 1)
+
+
+let rec pow_monotone (a:int) (b:int)
+    : Lemma (requires a >= 0 && b >= a)
+            (ensures pow2 a <= pow2 b)
+    = if a = 0 then ()
+      else pow_monotone (a - 1) (b - 1)
+
+
+let rec multpow_powsum (a:int) (b:int)
+    : Lemma (requires a >= 1 && b >= 1)
+            (ensures pow2 a * pow2 b = pow2 (a + b))
+    = if b > 2 then multpow_powsum a (b - 1)
+      else assert (pow2 a * pow2 2 = pow2 (a + 2))
+
+
+let sumpow_upper (a:int) (b:int)
+    : Lemma (requires a >= 1 && b >= 2 && a >= b)
+            (ensures pow2 a + pow2 b + 1 < pow2 (a * b))
+    = pow_monotone (a * 2) ( a * b);
+      assert (pow2 (a * 2) <= pow2 (a * b));
+      assert (pow2 (a + a) <= pow2 (a * 2));
+      multpow_powsum a a;
+      assert (pow2 a * pow2 a <= pow2 (a + a));
+      assert (4 <= pow2 a);
+      assert (4 * pow2 a <= pow2 a * pow2 a);
+      assert (pow2 a + pow2 a + pow2 a + pow2 a <= 4 * pow2 a);
+      pow_monotone b a;
+      assert (pow2 b <= pow2 a);
+      assert (pow2 a + pow2 b + 1 < pow2 a + pow2 a + pow2 a + pow2 a)
